P1.fsti
@@ -22,7 +22,6 @@ val append_left (#a: Type0) (ptr: t a) (v: a)
       (requires (fun h0 -> True))
       (ensures (fun h0 ptr' h1 -> v_linked_tree ptr' h1 == Spec.append_left (v_linked_tree ptr h0) v))
 
-
 /// Appends value [v] at the rightmost leaf of the tree that [ptr] points to.
 val append_right (#a: Type0) (ptr: t a) (v: a)
     : Steel (t a)
@@ -32,22 +31,6 @@ val append_right (#a: Type0) (ptr: t a) (v: a)
       (ensures (fun h0 ptr' h1 ->
         v_linked_tree ptr' h1 == Spec.append_right (v_linked_tree ptr h0) v
       ))
-(*)
-/// Returns the height of the tree that [ptr] points to
-val height (#a: Type0) (ptr: t a)
-    : Steel nat (linked_tree ptr) (fun _ -> linked_tree ptr)
-    (requires fun _ -> True)
-    (ensures fun h0 x h1 ->
-        v_linked_tree ptr h0 == v_linked_tree ptr h1 /\
-        Spec.height (v_linked_tree ptr h0) == x)
-
-/// Returns a boolean indicating whether element [v] belongs to the tree that [ptr] points to
-val member (#a: eqtype) (ptr: t a) (v: a)
-    : Steel bool (linked_tree ptr) (fun _ -> linked_tree ptr)
-    (requires fun _ -> True)
-    (ensures fun h0 b h1 ->
-        v_linked_tree ptr h0 == v_linked_tree ptr h1 /\
-        (Spec.mem (v_linked_tree ptr h0) v <==> b))
 
 (*** Rotation functions used internally to balance AVL trees ***)
 
@@ -64,6 +47,24 @@ val rotate_right (#a: Type) (ptr: t a)
     (ensures (fun h0 ptr' h1 ->
         Spec.rotate_right (v_linked_tree ptr h0) == Some (v_linked_tree ptr' h1)
     ))
+
+(*)
+/// Returns the height of the tree that [ptr] points to
+val height (#a: Type0) (ptr: t a)
+    : Steel nat (linked_tree ptr) (fun _ -> linked_tree ptr)
+    (requires fun _ -> True)
+    (ensures fun h0 x h1 ->
+        v_linked_tree ptr h0 == v_linked_tree ptr h1 /\
+        Spec.height (v_linked_tree ptr h0) == x)
+
+(*)
+/// Returns a boolean indicating whether element [v] belongs to the tree that [ptr] points to
+val member (#a: eqtype) (ptr: t a) (v: a)
+    : Steel bool (linked_tree ptr) (fun _ -> linked_tree ptr)
+    (requires fun _ -> True)
+    (ensures fun h0 b h1 ->
+        v_linked_tree ptr h0 == v_linked_tree ptr h1 /\
+        (Spec.mem (v_linked_tree ptr h0) v <==> b))
 
 val rotate_right_left (#a: Type) (ptr: t a)
     : Steel (t a) (linked_tree ptr) (fun ptr' -> linked_tree ptr')
